a small example with bind of atomic and ghost

pulse/examples/dsls/mini_steel/Pulse.Checker.Pure.fst
@@ -191,3 +191,16 @@ let check_vprop (f:RT.fstar_top_env)
     match ty with
     | Tm_VProp -> (| t, E d |)
     | _ -> T.fail "Expected a vprop"
+
+let get_non_informative_witness f g u t =
+  let err () = T.fail "non_informative_witness supported only for unit and prop" in
+  match t with
+  | Tm_FVar l ->
+    if l = R.unit_lid || l = R.prop_qn
+    then let w_lid = mk_steel_wrapper_lid
+                       (if l = R.unit_lid then "unit_non_informative"
+                        else "prop_non_informative") in
+         let e = Tm_FVar w_lid in
+         check_tot_with_expected_typ f g e (non_informative_witness_t u t)
+    else err ()
+  | _ -> err ()
